ulib/FStar.Modifies.fst
@@ -5,597 +5,215 @@ module HST = FStar.HyperStack.ST
 module B = FStar.Buffer
 module U32 = FStar.UInt32
 
-noeq
-type loc_aux : Type =
-  | LocBuffer:
-    (#t: Type) ->
-    (b: B.buffer t) ->
-    loc_aux
-  | LocUnion:
-    (l1: loc_aux) ->
-    (l2: loc_aux) ->
-    loc_aux
+type abuffer' = {
+  b_region: HS.rid;
+  b_addr: nat;
+  b_max_length: nat;
+  b_offset: nat;
+  b_length: nat;
+}
 
-let rec loc_aux_in_addr
-  (l: loc_aux)
-  (r: HS.rid)
-  (n: nat)
+type abuffer = (x: abuffer' { x.b_offset + x.b_length <= x.b_max_length } )
+
+let abuffer_of_buffer (#a: Type) (b: B.buffer a) : GTot abuffer = {
+  b_region = B.frameOf b;
+  b_addr = B.as_addr b;
+  b_max_length = B.max_length b;
+  b_offset = B.idx b;
+  b_length = B.length b;
+}
+
+let aloc (r: HS.rid) (a: nat) : Tot Type0 =
+  (x: abuffer { x.b_region == r /\ x.b_addr == a } )
+
+let abuffer_includes (larger smaller: abuffer) : GTot Type0 =
+  larger.b_region == smaller.b_region /\
+  larger.b_addr == smaller.b_addr /\
+  larger.b_max_length == smaller.b_max_length /\
+  larger.b_offset <= smaller.b_offset /\
+  smaller.b_offset + smaller.b_length <= larger.b_offset + larger.b_length
+
+let abuffer_disjoint (x1 x2: abuffer) : GTot Type0 =
+  (x1.b_region == x2.b_region /\ x1.b_addr == x2.b_addr) ==>
+  (x1.b_max_length == x2.b_max_length /\
+    (x1.b_offset + x1.b_length <= x2.b_offset \/
+     x2.b_offset + x2.b_length <= x1.b_offset))
+
+let abuffer_preserved
+  (x: abuffer)
+  (h1 h2: HS.mem)
 : GTot Type0
-  (decreases l)
-= match l with
-  | LocUnion l1 l2 -> loc_aux_in_addr l1 r n /\ loc_aux_in_addr l2 r n
-  | LocBuffer b ->
-    B.frameOf b == r /\
-    B.as_addr b == n
-
-noeq
-type loc' : Type =
-  | Loc:
-      (regions: Ghost.erased (Set.set HS.rid)) ->
-      (addrs: (
-	(r: HS.rid) ->
-	Ghost (Set.set nat)
-	(requires (Set.mem r (Ghost.reveal regions)))
-	(ensures (fun _ -> True))
-      )) ->
-      (aux_addrs: (
-	(r: HS.rid) ->
-	Ghost (Set.set nat)
-	(requires (Set.mem r (Ghost.reveal regions)))
-	(ensures (fun y -> Set.subset (Set.intersect y (addrs r)) Set.empty))
-      )) ->
-      (aux: (
-	(r: HS.rid) ->
-	(n: nat) ->
-	Ghost loc_aux
-	(requires (
-	  Set.mem r (Ghost.reveal regions) /\
-	  Set.mem n (aux_addrs r)
-	))
-	(ensures (fun y ->
-          loc_aux_in_addr y r n
-      )))) ->
-      loc'
-
-let loc = loc'
-
-let loc_none = Loc
-  (Ghost.hide (Set.empty))
-  (fun _ -> Set.empty)
-  (fun _ -> Set.empty)
-  (fun _ _ -> false_elim ())
-
-let regions_of_loc
-  (s: loc)
-: GTot (Set.set HS.rid)
-= Ghost.reveal (Loc?.regions s)
-
-let addrs_of_loc_weak
-  (l: loc)
-  (r: HS.rid)
-: GTot (Set.set nat)
-= if Set.mem r (regions_of_loc l)
-  then Loc?.addrs l r
-  else Set.empty
-
-let addrs_of_loc_aux
-  (l: loc)
-  (r: HS.rid)
-: GTot (Set.set nat)
-= if Set.mem r (regions_of_loc l)
-  then Loc?.aux_addrs l r
-  else Set.empty
-
-let addrs_of_loc
-  (l: loc)
-  (r: HS.rid)
-: GTot (Set.set nat)
-= Set.union
-    (addrs_of_loc_weak l r)
-    (addrs_of_loc_aux l r)
-
-let addrs_of_loc_aux_prop
-  (l: loc)
-  (r: HS.rid)
-: Lemma
-  (Set.subset (Set.intersect (addrs_of_loc_aux l r) (addrs_of_loc_weak l r)) Set.empty)
-  [SMTPatOr [
-    [SMTPat (addrs_of_loc_aux l r)];
-    [SMTPat (addrs_of_loc_weak l r)];
-    [SMTPat (addrs_of_loc l r)];
-  ]]
-= ()
-
-let loc_union s1 s2 =
-  if StrongExcludedMiddle.strong_excluded_middle (s1 == s2)
-  then s1
-  else
-  let regions1 = Ghost.reveal (Loc?.regions s1) in
-  let regions2 = Ghost.reveal (Loc?.regions s2) in
-  let regions = Set.union regions1 regions2 in
-  let addrs
-    (r: HS.rid)
-  : Ghost (Set.set nat)
-    (requires (Set.mem r regions))
-    (ensures (fun _ -> True))
-  = Set.union
-      (if Set.mem r regions1 then Loc?.addrs s1 r else Set.empty)
-      (if Set.mem r regions2 then Loc?.addrs s2 r else Set.empty)
-  in
-  let aux_addrs
-    (r: HS.rid)
-  : Ghost (Set.set nat)
-    (requires (Set.mem r regions))
-    (ensures (fun y -> Set.subset (Set.intersect y (addrs r)) Set.empty))
-  = Set.intersect
-      (Set.union (addrs_of_loc_aux s1 r) (addrs_of_loc_aux s2 r))
-      (Set.complement (addrs r))
-  in
-  let aux
-    (r: HS.rid)
-    (n: nat)
-  : Ghost loc_aux
-    (requires (Set.mem r regions /\ Set.mem n (aux_addrs r)))
-    (ensures (fun y -> loc_aux_in_addr y r n))
-  = let l1 =
-      if Set.mem r regions1 && Set.mem n (Loc?.aux_addrs s1 r)
-      then Some (Loc?.aux s1 r n)
-      else None
-    in
-    let l2 =
-      if Set.mem r regions2 && Set.mem n (Loc?.aux_addrs s2 r)
-      then Some (Loc?.aux s2 r n)
-      else None
-    in
-    match l1, l2 with
-    | Some l1, Some l2 -> LocUnion l1 l2
-    | Some l1, _ -> l1
-    | _, Some l2 -> l2
-  in
-  Loc
-    (Ghost.hide regions)
-    addrs
-    aux_addrs
-    aux
-
-let loc_union_idem s = ()
-
-let loc_buffer #t b =
-    Loc
-      (Ghost.hide (Set.singleton (B.frameOf b)))
-      (fun _ -> Set.empty)
-      (fun _ -> Set.singleton (B.as_addr b))
-      (fun _ _ -> LocBuffer b)
-
-let loc_addresses r n =
-  Loc
-    (Ghost.hide (Set.singleton r))
-    (fun _ -> n)
-    (fun _ -> Set.empty)
-    (fun _ _ -> false_elim ())
-
-let loc_regions r =
-  Loc
-    (Ghost.hide r)
-    (fun r' -> if Set.mem r' r then Set.complement Set.empty else Set.empty)
-    (fun _ -> Set.empty)
-    (fun _ _ -> false_elim ())
-
-let rec loc_aux_includes_buffer
-  (#a: Type)
-  (s: loc_aux)
-  (b: B.buffer a)
-: GTot Type0
-  (decreases s)
-= match s with
-  | LocUnion s1 s2 -> loc_aux_includes_buffer s1 b \/ loc_aux_includes_buffer s2 b
-  | LocBuffer #a0 b0 -> a == a0 /\ b0 `B.includes` b
-
-let rec loc_aux_includes
-  (s1 s2: loc_aux)
-: GTot Type0
-  (decreases s2)
-= match s2 with
-  | LocUnion s2l s2r -> loc_aux_includes s1 s2l /\ loc_aux_includes s1 s2r
-  | LocBuffer b -> loc_aux_includes_buffer s1 b
-
-let rec loc_aux_includes_union_l
-  (s1 s2 s: loc_aux)
-: Lemma
-  (requires (loc_aux_includes s1 s \/ loc_aux_includes s2 s))
-  (ensures (loc_aux_includes (LocUnion s1 s2) s))
-  (decreases s)
-= match s with 
-  | LocUnion sl sr -> loc_aux_includes_union_l s1 s2 sl; loc_aux_includes_union_l s1 s2 sr
-  | _ -> ()
-
-let rec loc_aux_includes_refl
-  (s: loc_aux)
-: Lemma
-  (loc_aux_includes s s)
-= match s with
-  | LocUnion sl sr ->
-    loc_aux_includes_refl sl;
-    loc_aux_includes_refl sr;
-    loc_aux_includes_union_l sl sr sl;
-    loc_aux_includes_union_l sl sr sr
-  | _ -> ()
-
-let loc_aux_includes_union_l_r
-  (s s': loc_aux)
-: Lemma
-  (loc_aux_includes (LocUnion s s') s)
-= loc_aux_includes_refl s;
-  loc_aux_includes_union_l s s' s
-
-let loc_aux_includes_union_l_l
-  (s s': loc_aux)
-: Lemma
-  (loc_aux_includes (LocUnion s' s) s)
-= loc_aux_includes_refl s;
-  loc_aux_includes_union_l s' s s
-
-let rec loc_aux_includes_buffer_includes
-  (#a: Type)
-  (s: loc_aux)
-  (b1 b2: B.buffer a)
-: Lemma
-  (requires (loc_aux_includes_buffer s b1 /\ b1 `B.includes` b2))
-  (ensures (loc_aux_includes_buffer s b2))
-  (decreases s)
-= match s with
-  | LocUnion sl sr ->
-    Classical.or_elim
-      #(loc_aux_includes_buffer sl b1)
-      #(loc_aux_includes_buffer sr b1)
-      #(fun _ -> loc_aux_includes_buffer s b2)
-      (fun _ -> loc_aux_includes_buffer_includes sl b1 b2)
-      (fun _ -> loc_aux_includes_buffer_includes sr b1 b2)
-  | _ -> ()
-
-let rec loc_aux_includes_loc_aux_includes_buffer
-  (#a: Type)
-  (s1 s2: loc_aux)
-  (b: B.buffer a)
-: Lemma
-  (requires (loc_aux_includes s1 s2 /\ loc_aux_includes_buffer s2 b))
-  (ensures (loc_aux_includes_buffer s1 b))
-  (decreases s2)
-= match s2 with
-  | LocUnion s2l s2r ->
-    Classical.or_elim
-      #(loc_aux_includes_buffer s2l b)
-      #(loc_aux_includes_buffer s2r b)
-      #(fun _ -> loc_aux_includes_buffer s1 b)
-      (fun _ -> loc_aux_includes_loc_aux_includes_buffer s1 s2l b)
-      (fun _ -> loc_aux_includes_loc_aux_includes_buffer s1 s2r b)
-  | LocBuffer b2 -> loc_aux_includes_buffer_includes s1 b2 b
-
-let rec loc_aux_includes_trans
-  (s1 s2 s3: loc_aux)
-: Lemma
-  (requires (loc_aux_includes s1 s2 /\ loc_aux_includes s2 s3))
-  (ensures (loc_aux_includes s1 s3))
-  (decreases s3)
-= match s3 with
-  | LocUnion s3l s3r ->
-    loc_aux_includes_trans s1 s2 s3l;
-    loc_aux_includes_trans s1 s2 s3r
-  | LocBuffer b -> loc_aux_includes_loc_aux_includes_buffer s1 s2 b
-
-(* the following is necessary because `decreases` messes up 2nd-order unification with `Classical.forall_intro_3` *)
-
-let loc_aux_includes_trans'
-  (s1 s2: loc_aux)
-  (s3: loc_aux)
-: Lemma
-  ((loc_aux_includes s1 s2 /\ loc_aux_includes s2 s3) ==> loc_aux_includes s1 s3)
-= Classical.move_requires (loc_aux_includes_trans s1 s2) s3
-
-let addrs_of_loc_weak_loc_union
-  (l1 l2: loc)
-  (r: HS.rid)
-: Lemma
-  (addrs_of_loc_weak (loc_union l1 l2) r == Set.union (addrs_of_loc_weak l1 r) (addrs_of_loc_weak l2 r))
-  [SMTPat (addrs_of_loc_weak (loc_union l1 l2) r)]
-= assert (Set.equal (addrs_of_loc_weak (loc_union l1 l2) r) (Set.union (addrs_of_loc_weak l1 r) (addrs_of_loc_weak l2 r)))
-
-let addrs_of_loc_union
-  (l1 l2: loc)
-  (r: HS.rid)
-: Lemma
-  (addrs_of_loc (loc_union l1 l2) r == Set.union (addrs_of_loc l1 r) (addrs_of_loc l2 r))
-  [SMTPat (addrs_of_loc (loc_union l1 l2) r)]
-= assert (Set.equal (addrs_of_loc (loc_union l1 l2) r) (Set.union (addrs_of_loc l1 r) (addrs_of_loc l2 r)))
-
-let loc_includes s1 s2 =
-  let regions1 = Ghost.reveal (Loc?.regions s1) in
-  let regions2 = Ghost.reveal (Loc?.regions s2) in (
-    Set.subset regions2 regions1 /\ (
-      forall (r: HS.rid) .
-      Set.subset (addrs_of_loc_weak s2 r) (addrs_of_loc_weak s1 r)
-    ) /\ (
-      forall (r: HS.rid) .
-      Set.subset (addrs_of_loc s2 r) (addrs_of_loc s1 r)
-    ) /\ (
-      forall (r: HS.rid) (n: nat) .
-      (Set.mem r regions2 /\ Set.mem n (addrs_of_loc_aux s2 r) /\ Set.mem n (addrs_of_loc_aux s1 r)) ==>
-      loc_aux_includes (Loc?.aux s1 r n) (Loc?.aux s2 r n)
+= (forall (t: Type) (b: B.buffer t) .
+    (
+      B.live h1 b /\
+      B.length b <> 0 /\
+      abuffer_of_buffer b == x
+    ) ==> (
+      B.live h2 b /\
+      B.as_seq h2 b == B.as_seq h1 b
   ))
 
-let loc_includes_refl s =
-  let pre
-    (r: HS.rid)
-    (n: nat)
-  : GTot Type0
-  = Set.mem r (regions_of_loc s) /\
-    Set.mem n (Loc?.aux_addrs s r)
-  in
-  let post
-    (r: HS.rid)
-    (n: nat)
-  : GTot Type0
-  = pre r n /\
-    loc_aux_includes (Loc?.aux s r n) (Loc?.aux s r n)
-  in
-  let f
-    (r: HS.rid)
-    (n: nat)
-  : Lemma
-    (requires (pre r n))
-    (ensures (post r n))
-  = loc_aux_includes_refl (Loc?.aux s r n)
-  in
-  Classical.forall_intro_2 (fun r -> Classical.move_requires (f r))
+module MG = FStar.ModifiesGen
 
-let loc_includes_trans s1 s2 s3 =
-  Classical.forall_intro_3 loc_aux_includes_trans'
+let cls = MG.Cls #aloc
+  (fun #r #a -> abuffer_includes)
+  (fun #r #a x -> ())
+  (fun #r #a x1 x2 x3 -> ())
+  (fun #r #a -> abuffer_disjoint)
+  (fun #r #a x1 x2 -> ())
+  (fun #r #a larger1 larger2 smaller1 smaller2 -> ())
+  (fun #r #a -> abuffer_preserved)
+  (fun #r #a x h -> ())
+  (fun #r #a x h1 h2 h3 -> ())
+  (fun #r #a b h1 h2 f ->
+    let g (t: Type0) (b' : B.buffer t) : Lemma
+      (requires (abuffer_of_buffer b' == b /\ B.live h1 b'))
+      (ensures (B.live h2 b' /\ B.as_seq h2 b' == B.as_seq h1 b'))
+    = f _ _ (B.content b')
+    in
+    let g' (t: Type0) (b' : B.buffer t) : Lemma
+      ((abuffer_of_buffer b' == b /\ B.live h1 b') ==>
+        (B.live h2 b' /\ B.as_seq h2 b' == B.as_seq h1 b'))
+    = Classical.move_requires (g t) b'
+    in
+    Classical.forall_intro_2 g'
+  )
+  (fun #r #a b h1 h2 -> ())
 
-let loc_includes_union_r s s1 s2 = ()
+let loc = MG.loc cls
 
-let loc_includes_union_l s1 s2 s =
-  let u12 = loc_union s1 s2 in
-  if StrongExcludedMiddle.strong_excluded_middle (s1 == s2)
-  then ()
-  else begin
-    Classical.forall_intro loc_aux_includes_refl;
-    Classical.forall_intro_2 loc_aux_includes_union_l_l;
-    Classical.forall_intro_2 loc_aux_includes_union_l_r;
-    Classical.or_elim
-      #(loc_includes s1 s)
-      #(loc_includes s2 s)
-      #(fun _ -> loc_includes (loc_union s1 s2) s)
-      (fun _ -> loc_includes_trans u12 s1 s)
-      (fun _ -> loc_includes_trans u12 s2 s)
-  end
+let loc_none = MG.loc_none
 
-let loc_includes_none s = ()
+let loc_union = MG.loc_union
 
-let loc_includes_buffer #t b1 b2 = ()
+let loc_union_idem = MG.loc_union_idem
+
+let loc_buffer #t b =
+  MG.loc_of_aloc #_ #cls #(B.frameOf b) #(B.as_addr b) (abuffer_of_buffer b)
+
+let loc_addresses = MG.loc_addresses
+
+let loc_regions = MG.loc_regions
+
+let loc_includes = MG.loc_includes
+
+let loc_includes_refl = MG.loc_includes_refl
+
+let loc_includes_trans = MG.loc_includes_trans
+
+let loc_includes_union_r = MG.loc_includes_union_r
+
+let loc_includes_union_l = MG.loc_includes_union_l
+
+let loc_includes_none = MG.loc_includes_none
+
+let loc_includes_buffer #t b1 b2 =
+  MG.loc_includes_aloc #_ #cls #(B.frameOf b1) #(B.as_addr b1) (abuffer_of_buffer b1) (abuffer_of_buffer b2)
 
 let loc_includes_gsub_buffer_r l #t b i len =
   loc_includes_trans l (loc_buffer b) (loc_buffer (B.sub b i len))
 
 let loc_includes_gsub_buffer_l #t b i1 len1 i2 len2 = ()
 
-let loc_includes_addresses_buffer #t r s p = ()
+let loc_includes_addresses_buffer #t r s p =
+  MG.loc_includes_addresses_aloc #_ #cls r s #(B.as_addr p) (abuffer_of_buffer p)
 
-let loc_includes_region_buffer #t s b = ()
+let loc_includes_region_buffer #t s b =
+  MG.loc_includes_region_aloc #_ #cls s #(B.frameOf b) #(B.as_addr b) (abuffer_of_buffer b)
 
-let loc_includes_region_addresses s r a = ()
+let loc_includes_region_addresses = MG.loc_includes_region_addresses #_ #cls
 
-let loc_includes_region_region s1 s2 = ()
+let loc_includes_region_region = MG.loc_includes_region_region #_ #cls
 
-#set-options "--z3rlimit 16"
+let loc_includes_region_union_l = MG.loc_includes_region_union_l
 
-let loc_includes_region_union_l l s1 s2 = ()
+let loc_disjoint = MG.loc_disjoint
 
-#reset-options
+let loc_disjoint_sym = MG.loc_disjoint_sym
 
+let loc_disjoint_none_r = MG.loc_disjoint_none_r
 
-(* Disjointness of two memory locations *)
+let loc_disjoint_union_r = MG.loc_disjoint_union_r
 
-let rec loc_aux_disjoint_buffer
-  (l: loc_aux)
-  (#t: Type)
-  (p: B.buffer t)
-: GTot Type0
-  (decreases l)
-= match l with
-  | LocUnion ll lr ->
-    loc_aux_disjoint_buffer ll p /\ loc_aux_disjoint_buffer lr p
-  | LocBuffer b -> B.disjoint b p
+let loc_disjoint_includes = MG.loc_disjoint_includes
 
-let rec loc_aux_disjoint
-  (l1 l2: loc_aux)
-: GTot Type0
-  (decreases l2)
-= match l2 with
-  | LocUnion ll lr ->
-    loc_aux_disjoint l1 ll /\ loc_aux_disjoint l1 lr
-  | LocBuffer b ->
-    loc_aux_disjoint_buffer l1 b
-
-let rec loc_aux_disjoint_union_l
-  (ll1 lr1 l2: loc_aux)
-: Lemma
-  (ensures (loc_aux_disjoint (LocUnion ll1 lr1) l2 <==> (loc_aux_disjoint ll1 l2 /\ loc_aux_disjoint lr1 l2)))
-  (decreases l2)
-= match l2 with
-  | LocUnion ll2 lr2 ->
-    loc_aux_disjoint_union_l ll1 lr1 ll2;
-    loc_aux_disjoint_union_l ll1 lr1 lr2
-  | _ -> ()
-
-let loc_aux_disjoint_union_r
-  (l1 ll2 lr2: loc_aux)
-: Lemma
-  (loc_aux_disjoint l1 (LocUnion ll2 lr2) <==> (loc_aux_disjoint l1 ll2 /\ loc_aux_disjoint l1 lr2))
-= ()
-
-let rec loc_aux_size
-  (l: loc_aux)
-: GTot nat
-= match l with
-  | LocUnion l1 l2 ->
-    let n1 = loc_aux_size l1 in
-    let n2 = loc_aux_size l2 in
-    1 + (if n1 > n2 then n1 else n2)
-  | _ -> 0
-
-let rec loc_aux_disjoint_sym
-  (l1 l2: loc_aux)
-: Lemma
-  (ensures (loc_aux_disjoint l1 l2 <==> loc_aux_disjoint l2 l1))
-  (decreases (loc_aux_size l1 + loc_aux_size l2))
-= match l2 with
-  | LocUnion ll lr ->
-    loc_aux_disjoint_union_r l1 ll lr;
-    loc_aux_disjoint_sym l1 ll;
-    loc_aux_disjoint_sym l1 lr;
-    loc_aux_disjoint_union_l ll lr l1
-  | _ ->
-    begin match l1 with
-    | LocUnion ll lr ->
-      loc_aux_disjoint_union_l ll lr l2;
-      loc_aux_disjoint_sym ll l2;
-      loc_aux_disjoint_sym lr l2;
-      loc_aux_disjoint_union_r l2 ll lr
-    | _ -> ()
-    end
-
-(* Same problem with decreases here *)
-
-let loc_aux_disjoint_sym'
-  (l1 l2: loc_aux)
-: Lemma
-  (loc_aux_disjoint l1 l2 <==> loc_aux_disjoint l2 l1)
-= loc_aux_disjoint_sym l1 l2
-
-let regions_of_loc_loc_union
-  (s1 s2: loc)
-: Lemma
-  (regions_of_loc (loc_union s1 s2) == regions_of_loc s1 `Set.union` regions_of_loc s2)
-  [SMTPat (regions_of_loc (loc_union s1 s2))]
-= assert (regions_of_loc (loc_union s1 s2) `Set.equal` (regions_of_loc s1 `Set.union` regions_of_loc s2))
-
-let regions_of_loc_monotonic
-  (s1 s2: loc)
-: Lemma
-  (requires (loc_includes s1 s2))
-  (ensures (Set.subset (regions_of_loc s2) (regions_of_loc s1)))
-= ()
-
-let loc_disjoint'
-  (l1 l2: loc)
-: GTot Type0
-= (forall (r: HS.rid) .
-      Set.subset (Set.intersect (addrs_of_loc_weak l1 r) (addrs_of_loc l2 r)) Set.empty /\
-      Set.subset (Set.intersect (addrs_of_loc l1 r) (addrs_of_loc_weak l2 r)) Set.empty
-  ) /\
-  (forall (r: HS.rid) (n: nat) .
-    (Set.mem r (regions_of_loc l1) /\ Set.mem n (addrs_of_loc_aux l1 r) /\
-     Set.mem r (regions_of_loc l2) /\ Set.mem n (addrs_of_loc_aux l2 r)) ==>
-    loc_aux_disjoint (Loc?.aux l1 r n) (Loc?.aux l2 r n)
-  )
-
-let loc_disjoint = loc_disjoint'
-
-let loc_disjoint_sym l1 l2 =
-  Classical.forall_intro_2 loc_aux_disjoint_sym'
-
-let loc_disjoint_none_r s = ()
-
-let loc_disjoint_union_r s s1 s2 = ()
-
-let rec loc_aux_disjoint_buffer_includes
-  (l: loc_aux)
-  (#t: Type)
-  (p1: B.buffer t)
-  (p2: B.buffer t)
-: Lemma
-  (requires (loc_aux_disjoint_buffer l p1 /\ p1 `B.includes` p2))
-  (ensures (loc_aux_disjoint_buffer l p2))
-  (decreases l)
-= match l with
-  | LocUnion ll lr ->
-    loc_aux_disjoint_buffer_includes ll p1 p2;
-    loc_aux_disjoint_buffer_includes lr p1 p2
-  | _ -> ()
-
-let rec loc_aux_disjoint_loc_aux_includes_buffer
-  (l1 l2: loc_aux)
-  (#t3: Type)
-  (b3: B.buffer t3)
-: Lemma
-  (requires (loc_aux_disjoint l1 l2 /\ loc_aux_includes_buffer l2 b3))
-  (ensures (loc_aux_disjoint_buffer l1 b3))
-  (decreases l2)
-= match l2 with
-  | LocUnion l2l l2r ->
-    Classical.or_elim
-      #(loc_aux_includes_buffer l2l b3)
-      #(loc_aux_includes_buffer l2r b3)
-      #(fun _ -> loc_aux_disjoint_buffer l1 b3)
-      (fun _ -> loc_aux_disjoint_loc_aux_includes_buffer l1 l2l b3)
-      (fun _ -> loc_aux_disjoint_loc_aux_includes_buffer l1 l2r b3)
-  | LocBuffer b2 -> loc_aux_disjoint_buffer_includes l1 b2 b3
-
-let rec loc_aux_disjoint_loc_aux_includes
-  (l1 l2 l3: loc_aux)
-: Lemma
-  (requires (loc_aux_disjoint l1 l2 /\ loc_aux_includes l2 l3))
-  (ensures (loc_aux_disjoint l1 l3))
-  (decreases l3)
-= match l3 with
-  | LocUnion ll3 lr3 ->
-    loc_aux_disjoint_loc_aux_includes l1 l2 ll3;
-    loc_aux_disjoint_loc_aux_includes l1 l2 lr3
-  | LocBuffer b3 ->
-    loc_aux_disjoint_loc_aux_includes_buffer l1 l2 b3
-
-let loc_disjoint_includes p1 p2 p1' p2' =
-  regions_of_loc_monotonic p1 p1';
-  regions_of_loc_monotonic p2 p2';
-  let pre = //A rather brutal way to force inlining of pre and post in VC of the continuation
-    (fun r n ->
-      Set.mem r (regions_of_loc p1') /\ Set.mem n (addrs_of_loc_aux p1' r) /\
-      Set.mem r (regions_of_loc p2') /\ Set.mem n (addrs_of_loc_aux p2' r))
-    <: Tot ((r:HS.rid) -> (n:nat) -> GTot Type0)
-  in
-  let post =
-    (fun r n ->
-       pre r n /\
-       loc_aux_disjoint (Loc?.aux p1' r n) (Loc?.aux p2' r n))
-    <: Tot ((r:HS.rid) -> (n:nat) -> GTot Type0)
-  in
-  let f
-    (r: HS.rid)
-    (n: nat)
-  : Lemma
-    (requires (pre r n))
-    (ensures (post r n))
-  = let l1 = Loc?.aux p1 r n in
-    let l2 = Loc?.aux p2 r n in
-    let l1' = Loc?.aux p1' r n in
-    let l2' = Loc?.aux p2' r n in
-    loc_aux_disjoint_loc_aux_includes l1 l2 l2';
-    loc_aux_disjoint_sym l1 l2';
-    loc_aux_disjoint_loc_aux_includes l2' l1 l1';
-    loc_aux_disjoint_sym l2' l1'
-  in
-  Classical.forall_intro_2 (fun r -> Classical.move_requires (f r))
-
-let loc_disjoint_buffer #t1 #t2 b1 b2 = ()
+let loc_disjoint_buffer #t1 #t2 b1 b2 =
+  MG.loc_disjoint_aloc_intro #_ #cls #(B.frameOf b1) #(B.as_addr b1) #(B.frameOf b2) #(B.as_addr b2) (abuffer_of_buffer b1) (abuffer_of_buffer b2)
 
 let loc_disjoint_gsub_buffer #t b i1 len1 i2 len2 = ()
 
-let loc_disjoint_addresses r1 r2 n1 n2 = ()
+let loc_disjoint_addresses = MG.loc_disjoint_addresses #_ #cls
 
-let loc_disjoint_buffer_addresses #t p r n = ()
+let loc_disjoint_buffer_addresses #t p r n =
+  MG.loc_disjoint_aloc_addresses_intro #_ #cls #(B.frameOf p) #(B.as_addr p) (abuffer_of_buffer p) r n
 
-let loc_disjoint_regions rs1 rs2 = ()
+let loc_disjoint_regions = MG.loc_disjoint_regions #_ #cls
 
+let modifies = MG.modifies
+
+let modifies_mreference_elim = MG.modifies_mreference_elim
+
+let modifies_buffer_elim #t1 b p h h' =
+  MG.modifies_aloc_elim #_ #cls #(B.frameOf b) #(B.as_addr b) (abuffer_of_buffer b) p h h'
+
+let modifies_refl = MG.modifies_refl
+
+let modifies_loc_includes = MG.modifies_loc_includes
+
+let modifies_trans = MG.modifies_trans
+
+let modifies_only_live_regions = MG.modifies_only_live_regions
+
+let no_upd_fresh_region = MG.no_upd_fresh_region
+
+let modifies_fresh_frame_popped = MG.modifies_fresh_frame_popped
+
+let modifies_loc_regions_intro = MG.modifies_loc_regions_intro #_ #cls
+
+let modifies_loc_addresses_intro = MG.modifies_loc_addresses_intro
+
+let modifies_ralloc_post = MG.modifies_ralloc_post #_ #cls
+
+let modifies_salloc_post = MG.modifies_salloc_post #_ #cls
+
+let modifies_free = MG.modifies_free #_ #cls
+
+let modifies_none_modifies = MG.modifies_none_modifies #_ #cls
+
+let modifies_buffer_none_modifies h1 h2 =
+  MG.modifies_intro loc_none h1 h2
+    (fun _ -> ())
+    (fun _ _ _ -> ())
+    (fun _ _ _ -> ())
+
+let modifies_0_modifies h1 h2 =
+  B.lemma_reveal_modifies_0 h1 h2;
+  MG.modifies_intro loc_none h1 h2
+    (fun _ -> ())
+    (fun _ _ _ -> ())
+    (fun _ _ _ -> ())
+
+(* Two live buffers at the same region and the same address have the
+same type.  Anyway this is a transitional library, and a new
+implementation is underway (see LowStar.Buffer) so don't give a sh*t,
+anyway this is F* code. *)
+
+#set-options "--z3rlimit 16"
+
+let modifies_1_modifies #a b h1 h2 =
+  B.lemma_reveal_modifies_1 b h1 h2;
+  MG.modifies_intro (loc_buffer b) h1 h2
+    (fun _ -> ())
+    (fun t' pre' b' ->
+      MG.loc_disjoint_sym (loc_mreference b') (loc_buffer b);
+      MG.loc_disjoint_aloc_addresses_elim #_ #cls #(B.frameOf b) #(B.as_addr b) (abuffer_of_buffer b) (HS.frameOf b') (Set.singleton (HS.as_addr b'))
+    )
+    (fun r' a' b' ->
+      assert (HS.modifies_ref (B.frameOf b) (Set.singleton (B.as_addr b)) h1 h2);
+      assert (B.live h1 b);
+      MG.loc_disjoint_aloc_elim #_ #cls #r' #a' #(B.frameOf b) #(B.as_addr b) b' (abuffer_of_buffer b)
+    )
+    
 
 (** The modifies clause proper *)
 
@@ -617,12 +235,13 @@ let modifies_preserves_buffers
   (h1 h2: HS.mem)
 : GTot Type0
 = (forall (t: Type) (b: B.buffer t) .
+    let s' = Ghost.reveal s in  
     let r = B.frameOf b in
     let a = B.as_addr b in (
       B.live h1 b /\
       B.length b <> 0 /\
       (Set.mem r (regions_of_loc s) ==> ~ (Set.mem a (addrs_of_loc_weak s r))) /\
-      ((Set.mem r (regions_of_loc s) /\ Set.mem a (addrs_of_loc_aux s r)) ==> loc_aux_disjoint_buffer (Loc?.aux s r a) b)
+      ((Set.mem r (Ghost.reveal (Loc?.aux_regions s')) /\ Set.mem a (Loc?.aux_addrs s' r)) ==> loc_aux_disjoint_buffer (Loc?.aux s' r a) (abuffer_of_buffer b))
     ) ==> (
       B.live h2 b /\
       B.as_seq h2 b == B.as_seq h1 b
@@ -639,7 +258,11 @@ let modifies = modifies'
 
 let modifies_mreference_elim #t #pre b p h h' = ()
 
+#set-options "--z3rlimit 16"
+
 let modifies_buffer_elim #t1 b p h h' = ()
+
+#reset-options
 
 let modifies_refl s h = ()
 
@@ -647,13 +270,11 @@ let loc_aux_disjoint_buffer_loc_aux_includes
   (l1: loc_aux)
 : Lemma
   (forall (l2: loc_aux)
-    (t3: Type)
-    (b3: B.buffer t3) .
+    (b3: abuffer) .
   (loc_aux_disjoint_buffer l1 b3 /\ loc_aux_includes l1 l2) ==> loc_aux_disjoint_buffer l2 b3)
 = let f
   (l2: loc_aux)
-  (t3: Type)
-  (b3: B.buffer t3)
+  (b3: abuffer)
   : Lemma
     (requires (loc_aux_disjoint_buffer l1 b3 /\ loc_aux_includes l1 l2))
     (ensures (loc_aux_disjoint_buffer l2 b3))
@@ -661,7 +282,7 @@ let loc_aux_disjoint_buffer_loc_aux_includes
     loc_aux_disjoint_loc_aux_includes (LocBuffer b3) l1 l2;
     loc_aux_disjoint_sym (LocBuffer b3) l2
   in
-  Classical.forall_intro_3 (fun (l2: loc_aux) (t3: Type) (b3: B.buffer t3) -> Classical.move_requires (f l2 t3) b3)
+  Classical.forall_intro_2 (fun (l2: loc_aux) (b3: abuffer) -> Classical.move_requires (f l2) b3)
 
 #set-options "--z3rlimit 32"
 
@@ -712,12 +333,15 @@ let restrict_to_regions
   (l: loc)
   (rs: Set.set HS.rid)
 : GTot loc
-= let (Loc regions addrs aux_addrs aux) = l in
-  Loc
-    (Ghost.hide (Set.intersect (Ghost.reveal regions) rs))
+= let (Loc whole_regions addr_regions addrs aux_regions aux_addrs aux) = Ghost.reveal l in
+  Ghost.hide (Loc
+    (Ghost.hide (Set.intersect (Ghost.reveal whole_regions) rs))
+    (Ghost.hide (Set.intersect (Ghost.reveal addr_regions) rs))
     (fun r -> addrs r)
+    (Ghost.hide (Set.intersect (Ghost.reveal aux_regions) rs))
     (fun r -> aux_addrs r)
     (fun r n -> aux r n)
+  )
 
 let regions_of_loc_restrict_to_regions
   (l: loc)
@@ -849,13 +473,15 @@ let modifies_buffer_none_modifies h1 h2 = ()
 let modifies_0_modifies h1 h2 =
   B.lemma_reveal_modifies_0 h1 h2
 
+#set-options "--z3rlimit 16"
+
 let modifies_1_modifies #a b h1 h2 =
   B.lemma_reveal_modifies_1 b h1 h2
 
 let modifies_2_modifies #a1 #a2 b1 b2 h1 h2 =
   B.lemma_reveal_modifies_2 b1 b2 h1 h2
 
-#set-options "--z3rlimit 32"
+#set-options "--z3rlimit 64"
 
 let modifies_3_modifies #a1 #a2 #a3 b1 b2 b3 h1 h2 =
   B.lemma_reveal_modifies_3 b1 b2 b3 h1 h2
@@ -867,138 +493,3 @@ let modifies_buffer_rcreate_post_common #a r init len b h0 h1 = ()
 let mreference_live_buffer_unused_in_disjoint #t1 #pre #t2 h b1 b2 = ()
 
 let buffer_live_mreference_unused_in_disjoint #t1 #t2 #pre h b1 b2 = ()
-
-
-let does_not_contain_addr' (h: HS.mem) (ra: HS.rid * nat) : GTot Type0 =
-  forall (a: Type) (rel: Preorder.preorder a) (r: HS.mreference a rel) . {:pattern (h `HS.contains` r) } (HS.frameOf r == fst ra /\ HS.as_addr r == snd ra /\ h `HS.contains` r) ==> False
-
-let does_not_contain_addr = does_not_contain_addr'
-
-let not_live_region_does_not_contain_addr h ra = ()
-
-let unused_in_does_not_contain_addr h #a #rel r = ()
-
-let addr_unused_in_does_not_contain_addr h ra = ()
-
-let free_does_not_contain_addr #a #rel r m x = ()
-
-let does_not_contain_addr_elim #a #rel r m x = ()
-
-#set-options "--z3rlimit 32"
-
-let modifies_only_live_addresses_weak
-  (r: HS.rid)
-  (a: Set.set nat)
-  (l: loc)
-  (h h' : HS.mem)
-: Lemma
-  (requires (
-    modifies (loc_union (loc_addresses r a) l) h h' /\
-    loc_disjoint (loc_addresses r a) l /\
-    (forall x . Set.mem x a ==> h `does_not_contain_addr` (r, x))
-  ))
-  (ensures (modifies l h h'))
-= assert (modifies_preserves_mreferences l h h')
-
-#reset-options
-
-(* Restrict a set of locations along a set of addresses in a given region *)
-
-let restrict_to_addresses
-  (l: loc)
-  (r: HS.rid)
-  (as: Set.set nat)
-: Ghost loc
-  (requires (loc_region_only r `loc_includes` l))
-  (ensures (fun _ -> True))
-= let (Loc regions addrs aux_addrs aux) = l in
-  let aux_addrs' = if Set.mem r (Ghost.reveal regions) then Set.intersect (aux_addrs r) as else Set.empty in
-    Loc
-      (Ghost.hide (Set.intersect (Ghost.reveal regions) (Set.singleton r)))
-      (fun _ -> if Set.mem r (Ghost.reveal regions) then Set.intersect (addrs r) as else Set.empty)
-      (fun _ -> aux_addrs')
-      (fun r n -> aux r n)
-
-let regions_of_loc_restrict_to_addresses
-  (l: loc)
-  (r: HS.rid)
-  (as: Set.set nat)
-: Lemma
-  (requires (loc_region_only r `loc_includes` l))
-  (ensures (regions_of_loc (restrict_to_addresses l r as) == Set.intersect (regions_of_loc l) (Set.singleton r)))
-  [SMTPat (regions_of_loc (restrict_to_addresses l r as))]
-= assert (regions_of_loc (restrict_to_addresses l r as) `Set.equal` Set.intersect (regions_of_loc l) (Set.singleton r))
-
-let addrs_of_loc_weak_restrict_to_addresses
-  (l: loc)
-  (r: HS.rid)
-  (as: Set.set nat)
-  (r' : HS.rid)
-: Lemma
-  (requires (loc_region_only r `loc_includes` l))
-  (ensures (addrs_of_loc_weak (restrict_to_addresses l r as) r' == (if r = r' then Set.intersect (addrs_of_loc_weak l r) as else Set.empty)))
-  [SMTPat (addrs_of_loc_weak (restrict_to_addresses l r as) r')]
-= assert (addrs_of_loc_weak (restrict_to_addresses l r as) r `Set.equal` Set.intersect (addrs_of_loc_weak l r) as)
-
-let addrs_of_loc_restrict_to_addresses
-  (l: loc)
-  (r: HS.rid)
-  (as: Set.set nat)
-  (r' : HS.rid)
-: Lemma
-  (requires (loc_region_only r `loc_includes` l))
-  (ensures (addrs_of_loc (restrict_to_addresses l r as) r' == (if r = r' then Set.intersect (addrs_of_loc l r) as else Set.empty)))
-  [SMTPat (addrs_of_loc (restrict_to_addresses l r as) r')]
-= assert (addrs_of_loc (restrict_to_addresses l r as) r `Set.equal` Set.intersect (addrs_of_loc l r) as);
-  assert (r <> r' ==> addrs_of_loc (restrict_to_addresses l r as) r' `Set.equal` Set.empty)
-
-let loc_includes_restrict_to_addresses
-  (l: loc)
-  (r: HS.rid)
-  (as: Set.set nat)
-: Lemma
-  (requires (loc_region_only r `loc_includes` l))
-  (ensures (loc_includes l (restrict_to_addresses l r as)))
-= Classical.forall_intro loc_aux_includes_refl
-
-#set-options "--z3rlimit 10"
-let loc_includes_loc_union_restrict_to_addresses
-  (l: loc)
-  (r: HS.rid)
-  (as: Set.set nat)
-: Lemma
-  (requires (loc_region_only r `loc_includes` l))
-  (ensures (loc_includes (loc_union (restrict_to_addresses l r as) (restrict_to_addresses l r (Set.complement as))) l))
-= Classical.forall_intro loc_aux_includes_refl
-
-let loc_includes_loc_addresses_restrict_to_addresses
-  (l: loc)
-  (r: HS.rid)
-  (as: Set.set nat)
-: Lemma
-  (requires (loc_region_only r `loc_includes` l))
-  (ensures (loc_includes (loc_addresses r as) (restrict_to_addresses l r as)))
-= Classical.forall_intro loc_aux_includes_refl
-
-#set-options "--z3rlimit 64"
-
-let modifies_only_live_addresses r a l h h' =
-  let l_r = restrict_to_regions l (Set.singleton r) in
-  let l_not_r = restrict_to_regions l (Set.complement (Set.singleton r)) in
-  let l_a = restrict_to_addresses l_r r a in
-  let l_r_not_a = restrict_to_addresses l_r r (Set.complement a) in
-  let l_not_a = loc_union l_r_not_a l_not_r in
-  let l' = loc_union (loc_addresses r a) l_not_a in
-  loc_includes_loc_addresses_restrict_to_addresses l_r r a;
-  loc_includes_loc_union_restrict_to_regions l (Set.singleton r);
-  loc_includes_loc_union_restrict_to_addresses l_r r a;
-  loc_includes_trans (loc_union (loc_union l_a l_r_not_a) l_not_r) (loc_union l_r l_not_r) l;
-  loc_includes_trans (loc_union l_a l_not_a) (loc_union (loc_union l_a l_r_not_a) l_not_r) l;
-  loc_includes_trans l' (loc_union l_a l_not_a) l;
-  modifies_loc_includes (loc_union (loc_addresses r a) l_not_a) h h' (loc_union (loc_addresses r a) l);
-  modifies_only_live_addresses_weak r a l_not_a h h';
-  loc_includes_restrict_to_regions l (Set.complement (Set.singleton r));
-  loc_includes_restrict_to_addresses l_r r (Set.complement a);
-  modifies_loc_includes l h h' l_not_a
-
-#reset-options
